Get rid of the State.fsti file
This was preventing easy compliation to ocaml

tryf/Quint.State.fst
@@ -7,16 +7,42 @@ open FStar.List.Tot
 open Quint.Util
 open Quint.Ordered
 open Quint.State.Sig
+open Quint.Rng.Ops
 
 module DM = FStar.DependentMap
 module List = FStar.List.Tot
 module Rng = Quint.Rng
 module Set = Quint.Set
 
+/// # State
+
+let optional #k : (k -> Type) -> k -> Type =
+  fun f v -> option (f v)
+
+// TODO Find a way to abstract implementation of this so we don't have to expose the
+// dep map impl.
+/// A state defined by a signature `sig`
+let state {| s:sig |} = DM.t vars (optional s.types)
+
+/// Predicates over states
+let is_assigned {| sig |} (m:state) k = Some? (DM.sel m k)
+let is_unassigned {| sig |} (m:state) k = None? (DM.sel m k)
+let is_fresh {| sig |} (m:state) = forall (v:vars). is_unassigned m v
+let is_updated {| sig |} (m:state) = forall (v:vars). is_assigned m v
+
 let init_opt {| sig |}: f:(v:vars -> types v) -> v':vars -> option (types v') =
   fun init variable -> Some (init variable)
 
+/// A state initialization function
+type init_t {|sig|} = v:vars -> types v
+
+/// Construct a state from an initialization function
+val init : sig -> init_t -> s:state{is_updated s}
 let init (s:sig) (f:init_t) : state = DM.create (init_opt f)
+
+let empty_state {| sig |} : m:state{is_fresh m} =
+  let clear _ = None in
+  DM.create (clear)
 
 let upd {| sig |} (v:vars) (x:types v)
   : m:state{is_unassigned m v} -> m':state{is_assigned m' v} =
@@ -65,10 +91,38 @@ let rec append_mem #t l1 l2 a = match l1 with
   | [] -> ()
   | hd::tl -> append_mem tl l2 a
 
+/// # State functions: the *read* effect
+
+// TODO Use `DM.restrict` to limit map to just declared variables
+// A computation of `a` that can read from `state #sig`
+// TODO Figure out how to hide and abstract these
+let state_has {|sig|} (s:state) (vs:list vars) =
+    forall v. mem v vs ==> is_assigned s v
+
+let state_not_has {|sig|} (s:state) (vs:list vars) =
+    forall v. mem v vs ==> is_unassigned s v
+
+let if_state_has_all_it_is_updated
+    {|sig|}
+    (s:state)
+    (vs:list vars)
+    : Lemma ((state_has s vs /\ (forall (v:vars). mem v vs)) ==> is_updated s)
+    // [SMTPat (state_has s vs); SMTPat (is_updated s)]
+    = ()
+
+/// A computation of a value of type `a`,
+/// over a state defined by `sig`
+/// that can read from the variables in `list vars`
+type read {|sig|} (vs:list vars) (a:Type)
+  = s:state{state_has s vs} -> a
+
 let read_map {|sig|} #a #b #vs (f:a -> b) (x:read vs a) : read vs b
   = fun s -> f (x s)
 
+/// Puts a value of type `a` in a `read` context
+val pure {|sig|} #a #vs (x:a) : read vs a
 let pure {|sig|} #a #vs (x:a) : read vs a = fun _ -> x
+
 
 // This is what the monadic bindings would look like
 // but the read effect is only applicative!
@@ -80,14 +134,38 @@ let pure {|sig|} #a #vs (x:a) : read vs a = fun _ -> x
 //   (x : read vs a) (y : read vs' b) : read (vs @ vs') (a * b)
 //   = fun s -> (x s, y s)
 
+/// Read a value of type `types v`
+val ( ! ) {| sig |} : v:vars -> read [v] (types v)
 let ( ! ) {| sig |} (v:vars) : read [v] (types v) // s:state{is_assigned s v} -> types v
     =
     fun state -> Some?.v (DM.sel state v)
 
+/// Bind a computation of `a` from a read context that computes a `b`
+///
+/// E.g., if `X` is a state variable
+///
+/// ```
+/// let ex_1 : read [X] int =
+///   let! x = !X in
+///   x + 1
+/// ```
+val (let!) {|sig|} #a #b #vs : read vs a -> (a -> b) -> read vs b
 let (let!) {|sig|} #a #b #vs
   (x : read vs a) (f : a -> b) : read vs b
   = fun s -> (pure #_ #_ #vs (f (x s))) s
 
+/// Applicative binding of computationr within a read context
+///
+/// E.g.,
+///
+/// ```
+/// let ex_2 : read [X; V] bool =
+///   let! v = !V
+///   and! x = !X
+///   in
+///   v < 1 && x = "foo"
+/// ```
+val (and!) {|sig|} #a #b #vs #vs' : read vs a -> read vs' b -> read (vs @ vs') (a * b)
 let (and!) {|sig|} #a #b #vs #vs'
   (x : read vs a) (y : read vs' b) : read (vs @ vs') (a * b)
   = fun s -> (x s, y s)
@@ -98,14 +176,47 @@ let _read_ex : read [X; V] (int * string) =
     in
     (x, v)
 
+/// # State predicates: the *action* effect
+
+/// A state predicate, i.e., an action
+///
+/// An action over the state defined by `sig`
+/// that updates the variables `vars`
+///
+/// - `s0` is the current state
+/// - `s` is the intermediate state to be updated (lets us ensure no state is updated twice)
+/// - `s1` is the next state specified by by the action
+type action {|sig|} (vs:list vars)
+  = s0:state{is_updated s0}
+    -> option (
+      s:state{state_not_has s vs}
+      -> s1:state{state_has s1 vs /\ (forall v. (not (mem v vs)) ==> DM.sel s1 v == DM.sel s v)}
+    )
+
+/// Requirements
+val req {| sig |} #vs : read vs bool -> action []
 let req {| sig |} #vs : read vs bool -> action [] =
   fun r s0 ->
   if r s0 then Some (fun x -> x) else None
 
+let chk {|sig|} (b:bool): action [] =
+    fun s0 ->
+    if b then
+      Some (fun s -> s)
+    else
+      None
 
+/// `v @= x` updates the state variable `v` to the value `x` in the next state
+val ( @= ) {|sig|} : v:vars -> x:types v -> action [v]
 let ( @= ) {|sig|} (v:vars) (x:types v) : action [v]
   = fun _ -> Some (fun s -> upd v x s)
 
+// TODO: replace ! with @ for consistency
+/// The composition of actions
+val ( &! ) {|sig|} #vs #vs'
+  :  a1:action vs
+  -> a2:action vs'{forall v. mem v vs' ==> not (mem v vs)}
+  -> action (vs @ vs')
 /// Conjunction is the composition of actions
 let ( &! ) {|sig|} #vs #vs'
   (a1:action vs)
@@ -121,6 +232,8 @@ let ( &! ) {|sig|} #vs #vs'
   | Some upd2 ->
   Some (fun (s:state{state_not_has s (vs @ vs')}) -> (upd2 (upd1 s)))
 
+/// The alternation of actions
+val ( |! ) {|sig|} #vs : action vs -> action vs -> action vs
 // TODO Add non-det
 let ( |! ) {|sig|} #vs (a1:action vs) (a2:action vs) : action vs  =
   fun s0 ->
@@ -130,8 +243,65 @@ let ( |! ) {|sig|} #vs (a1:action vs) (a2:action vs) : action vs  =
   a2 s0
 
 
+/// # Data nondetermism: the *nondet* effect
+
+/// A computation of a value of type `a` in a nondet context
+type nondet (a:Type) = Rng.t a
+
+/// Nondeterministically select a value of type `a` from a non-empty set
+val one_of #a {|ordered a|} : Set.non_empty a -> nondet a
 let one_of #a {|ordered a|} (s:Set.non_empty a) : nondet a =
   Rng.rand_choice s.ls
+
+open Quint.Ordered
+
+module Set = Quint.Set
+
+/// # Transitions
+
+// A transition is an action that updates all the variables
+type transition {|sig|} #vs = a:action vs{(forall (v : vars). mem v vs)}
+
+let apply_det {|s:sig|} #vs
+  (t:transition #s #vs)
+  (s0:state{is_updated s0})
+  : option (s1:state{state_has s1 vs})
+   =
+  match t s0 with
+  | None -> None
+  | Some update ->
+  Some (update empty_state)
+
+
+/// Apply a transition to the state
+let apply {|s:sig|} #vs
+  (nt:nondet (transition #s #vs))
+  (s0:state{is_updated s0})
+  : nondet (option (s1:state{state_has s1 vs}))
+  =
+  let? t = nt in
+  apply_det t s0
+
+let rec run_aux {|s:sig|} #vs
+  (nt:nondet (transition #s #vs))
+  (s0:state{is_updated s0})
+  : nat -> nondet (list state)
+  = function
+  | 0 -> return []
+  | n ->
+  apply nt s0 >>= (function
+  | None    -> return []
+  | Some s1 ->
+  let? states = run_aux nt s0 (n - 1) in
+  s0 :: states)
+
+/// Run a transition for n_steps, or until it deadlocks
+let run {|s:sig|} #vs
+  (n_steps:nat)
+  (i:init_t)
+  (nt:nondet (transition #s #vs)) =
+  let s0 = init s i in
+  run_aux nt s0 n_steps
 
 // TODO: need to adjust precedence so don't need to use brackets
 let _ex_conj_action : transition =
